theories/rules/mov.v
@@ -8,21 +8,20 @@ Section mov.
 
 Context `{vmG: !gen_VMG Σ}.
   
-Lemma mov_word {E instr i qi w1 w3 q p} a w2 ra :
+Lemma mov_word {E instr i w1 w3 q p} a w2 ra :
   instr = Mov ra (inl w2) ->
   decode_instruction w1 = Some(instr) ->
   addr_in_page a p ->
-  {SS{{ ▷ (<<i>>{ qi }) ∗ ▷ (PC @@ i ->r a)
+  {SS{{  ▷ (PC @@ i ->r a)
           ∗ ▷ (a ->a w1) ∗ ▷ (A@i:={q} p)
           ∗ ▷ (ra @@ i ->r w3)}}}
     ExecI @ i ; E
-  {{{ RET ExecI; <<i>>{ qi }
-                   ∗ PC @@ i ->r (a ^+ 1)%f
+  {{{ RET ExecI;  PC @@ i ->r (a ^+ 1)%f
                    ∗ a ->a w1
                    ∗ A@i:={q} p
                    ∗ ra @@ i ->r w2 }}}.
 Proof.
-  iIntros (Hinstr Hdecode Hin ϕ) "(? & >Hpc & >Hapc & >Hacc & >Hra) Hϕ".
+  iIntros (Hinstr Hdecode Hin ϕ) "( >Hpc & >Hapc & >Hacc & >Hra) Hϕ".
   iApply (sswp_lift_atomic_step ExecI);[done|].
   iIntros (σ1) "%Hsche Hσ".
   inversion Hsche as [ Hcur ]; clear Hsche.
